src/Transforms/Shallow.dfy
@@ -11,7 +11,6 @@ module Bootstrap.Transforms.Shallow {
       function method {:opaque} Map_Method(m: Method, tr: ExprTransformer) : (m': Method)
         requires Shallow.All_Method(m, tr.f.requires)
         ensures Shallow.All_Method(m', tr.post) // FIXME Deep
-        ensures tr.rel(m.methodBody, m'.methodBody)
       {
         match m {
           case Method(CompileName, methodBody) =>
@@ -22,7 +21,6 @@ module Bootstrap.Transforms.Shallow {
       function method {:opaque} Map_Program(p: Program, tr: ExprTransformer) : (p': Program)
         requires Shallow.All_Program(p, tr.f.requires)
         ensures Shallow.All_Program(p', tr.post)
-        ensures tr.rel(p.mainMethod.methodBody, p'.mainMethod.methodBody)
       {
         match p {
           case Program(mainMethod) => Program(Map_Method(mainMethod, tr))
